src/dafny/beacon/statetransition/StateTransition.dfy
@@ -24,7 +24,9 @@ include "../BeaconChainTypes.dfy"
 include "../validators/Validators.dfy"
 include "../attestations/AttestationsTypes.dfy"
 include "../Helpers.dfy"
+include "../Helpers.s.dfy"
 include "StateTransition.s.dfy"
+include "StateTransition.p.dfy"
 include "../attestations/AttestationsHelpers.dfy"
 include "EpochProcessing.dfy"
 include "ProcessOperations.dfy"
@@ -47,53 +49,16 @@ module StateTransition {
     import opened AttestationsTypes
     import opened Helpers
     import opened BeaconHelpers
+    import opened BeaconHelperSpec
     import opened StateTransitionSpec
+    import opened StateTransitionProofs
     import opened AttestationsHelpers
     import opened EpochProcessing
     import opened ProcessOperations
     import opened ProcessOperationsSpec
     import opened Math
 
-    /**
-     *  Whether a block is valid in a given state.
-     *
-     *  @param  s   A beacon state.
-     *  @param  b   A block.
-     *
-     *  @returns    true iff `b` can be successfully added to the state `s`.
-     */
-    predicate isValidBlock(s : BeaconState, b : BeaconBlock) 
-    {
-        //  The block slot should be in the future.
-        s.slot < b.slot 
-        //  Fast forward s to b.slot and check `b` can be attached to the
-        //  resulting state's latest_block_header.
-        //  Check that number of deposits in b.body can be processed
-        && s.eth1_deposit_index as int + |b.body.deposits| < 0x10000000000000000  
-        && |s.validators| + |b.body.deposits| <= VALIDATOR_REGISTRY_LIMIT as int
-        // note that |b.body.deposits| is larger than required, only existing + new validators need to obey this bound
-        && total_balances(s.balances) + total_deposits(b.body.deposits) < 0x10000000000000000
-        // note that the |b.body.deposits| and total_deposits should refer to valid deposits
-        && |s.validators| == |s.balances|
-        && |s.eth1_data_votes| < EPOCHS_PER_ETH1_VOTING_PERIOD as int * SLOTS_PER_EPOCH as int
-        // && b.parent_root == 
-        //     hash_tree_root(
-        //         forwardStateToSlot(nextSlot(s), 
-        //         b.slot
-        //     ).latest_block_header) 
-        // //  Check that the block provides the correct hash for the state.
-        // &&  b.state_root == hash_tree_root(
-        //         updateDeposits(
-        //             updateEth1Data(
-        //                 addBlockToState(
-        //                     forwardStateToSlot(nextSlot(s), b.slot), 
-        //                     b
-        //                 ),
-        //                 b.body),
-        //             b.body.deposits
-        //         )
-        //     )
-    }
+    
 
     /**
      *  Compute the state obtained after adding a block.
@@ -365,48 +330,7 @@ module StateTransition {
         assert s' == updateBlock(s, b);
     }
 
-    /** */
-    function updateBlock(s: BeaconState, b: BeaconBlock): BeaconState
-        requires b.slot == s.slot
-        requires b.parent_root == hash_tree_root(s.latest_block_header)
-        requires s.eth1_deposit_index as int + |b.body.deposits| < 0x10000000000000000  
-        requires |s.eth1_data_votes| < EPOCHS_PER_ETH1_VOTING_PERIOD as int * SLOTS_PER_EPOCH as int
-        requires |s.validators| == |s.balances|
-        requires |s.validators| + |b.body.deposits| <= VALIDATOR_REGISTRY_LIMIT as int
-        requires total_balances(s.balances) + total_deposits(b.body.deposits) < 0x10000000000000000
-        requires |get_active_validator_indices(s.validators, get_current_epoch(s))| > 0
-        requires isValidBeaconBlockBody(s, b.body)
-
-        // ensures updateBlock(s,b).slot == b.slot
-        // ensures updateBlock(s,b).latest_block_header == BeaconBlockHeader(b.slot, b.proposer_index, b.parent_root, DEFAULT_BYTES32)
-        // ensures |updateBlock(s,b).validators| == |updateBlock(s,b).balances|
-        //ensures updateBlock(s,b) == updateOperations(updateEth1Data(updateRandao(addBlockToState(s, b), b.body), b.body), b.body)
-        
-    {
-        //  Start by creating a block header from the ther actual block.
-        var s1 := addBlockToState(s, b); 
-        assert s1 == addBlockToState(s, b);
-        assert (s1.balances == s.balances);
-        assert (s1.validators == s.validators);
-        
-        var s2 := updateRandao(s1, b.body);
-        assert s2 == updateRandao(addBlockToState(s, b), b.body);
-        assert (s2.balances == s.balances);
-        assert (s2.validators == s.validators);
-        
-        var s3 := updateEth1Data(s2, b.body);
-        assert (s3.balances == s.balances);
-        assert (s3.validators == s.validators);
-        assert |s3.validators| == |s3.balances|;
-        assert s3 == updateEth1Data(updateRandao(addBlockToState(s, b), b.body), b.body);
-
-        assert |get_active_validator_indices(s3.validators, get_current_epoch(s3))| > 0;
-        assume isValidBeaconBlockBody(s3, b.body);
-        
-        var s4 := updateOperations(s3, b.body);
-        assert s4 == updateOperations(updateEth1Data(updateRandao(addBlockToState(s, b), b.body), b.body), b.body);
-        s4
-    }
+    
 
     /**
      *  Check whether a block is valid and prepare and initialise new state
@@ -502,160 +426,6 @@ module StateTransition {
         }
             
 
-    }
-    
-
-    // // /**
-    // //  *  Process the operations defined by a block body.
-    // //  *  
-    // //  *  @param  s   A state.
-    // //  *  @param  bb  A block body.
-    // //  *  @returns    The state obtained after applying the operations of `bb` to `s`.
-    // //  */
-    // // method process_operations(s: BeaconState, bb: BeaconBlockBody)  returns (s' : BeaconState) 
-    // //     requires s.eth1_deposit_index as int +  |bb.deposits| < 0x10000000000000000 
-    // //     requires |s.validators| + |bb.deposits| <= VALIDATOR_REGISTRY_LIMIT as int
-    // //     requires |s.validators| == |s.balances|
-    // //     requires total_balances(s.balances) + total_deposits(bb.deposits) < 0x10000000000000000 
-        
-    // //     //ensures |s'.validators| == |s'.balances|
-    // //     ensures s' == updateDeposits(s, bb.deposits)
-    // //     ensures s'.slot == s.slot
-    // //     ensures s'.latest_block_header == s.latest_block_header
-    // //     //ensures s'.validators == s.validators + get_new_validators(s, [], bb.deposits)
-    // //     //ensures false
-    // // {
-    // //     //  process deposits in the beacon block body.
-    // //     s':= s;
-
-    // //     var i := 0;
-    // //     assert s' == updateDeposits(s, bb.deposits[..i]);
-    // //     assert total_balances(s'.balances) + total_deposits(bb.deposits[..i]) < 0x10000000000000000 ;
-        
-    // //     while i < |bb.deposits| 
-    // //         decreases |bb.deposits| - i
-
-    // //         invariant 0 <= i <= |bb.deposits|
-    // //         invariant s'.eth1_deposit_index == s.eth1_deposit_index + i as uint64
-            
-    // //         invariant total_balances(s.balances) + total_deposits(bb.deposits[..i]) < 0x10000000000000000 
-    // //         //invariant s'.validators == updateDeposits(s, bb.deposits[..i]).validators
-    // //         //invariant s'.balances == updateDeposits(s, bb.deposits[..i]).balances
-            
-    // //         //invariant total_balances(updateDeposits(s,bb.deposits[..i]).balances) == total_balances(s.balances) + total_deposits(bb.deposits[..i]) < 0x10000000000000000
-            
-    // //         //invariant s'.slot == s.slot 
-    // //         //invariant s'.latest_block_header == s.latest_block_header
-    // //         //invariant s'.block_roots == s.block_roots
-    // //         //invariant s'.state_roots == s.state_roots
-
-    // //         //invariant |s'.validators| == |s'.balances| 
-    // //         //invariant |s'.validators| <= |s.validators| + i
-    // //         //invariant |s.validators| + i <= VALIDATOR_REGISTRY_LIMIT as int
-    // //         invariant s' == updateDeposits(s, bb.deposits[..i])
-    // //         invariant s'.slot == s.slot
-    // //         invariant s'.latest_block_header == s.latest_block_header
-    // //         //invariant |bb.deposits[..i]| == i
-
-    // //         //invariant |s'.validators| <= |updateDeposits(s,bb.deposits[..i]).validators| <= |s'.validators| + i 
-    // //     {
-    // //         assert bb.deposits[..i+1] == bb.deposits[..i] + [bb.deposits[i]];
-
-    // //         s':= process_attestation(s', bb.attestations);
-
-    // //         //assert total_balances(updateDeposits(s, bb.deposits[..i]).balances) + bb.deposits[i].data.amount as int == total_balances(s.balances) + total_deposits(bb.deposits[..i]) + bb.deposits[i].data.amount as int;
-    // //         //assert total_deposits(bb.deposits[..i]) + bb.deposits[i].data.amount as int == total_deposits(bb.deposits[..i+1]);
-    // //         //assert total_balances(updateDeposits(s, bb.deposits[..i]).balances) + bb.deposits[i].data.amount as int == total_balances(s.balances) + total_deposits(bb.deposits[..i+1]);
-    // //         //assert i + 1  <= |bb.deposits|;
-    // //         subsetDepositSumProp(bb.deposits, i+1);
-    // //         //assert total_deposits(bb.deposits[..i+1]) <= total_deposits(bb.deposits);
-    // //         //assert total_balances(updateDeposits(s, bb.deposits[..i]).balances) + bb.deposits[i].data.amount as int < 0x10000000000000000;
-
-    // //         //assert updateDeposit(updateDeposits(s, bb.deposits[..i]),bb.deposits[i]) == updateDeposits(s, bb.deposits[..i+1]);
-            
-    // //         s':= process_deposit(s', bb.deposits[i]); 
-    // //         i := i+1;
-
-    // //     }
-    // //     assert bb.deposits[..i] == bb.deposits;
-
-    // // }
-
-    // /**
-    //  *  Process a deposit operation.
-    //  *
-    //  *  @param  s   A state.
-    //  *  @param  d   A deposit.  
-    //  *  @returns    The state obtained depositing of `d` to `s`.
-    //  *  @todo       Finish implementation of this function.
-    //  */
-    // method process_deposit(s: BeaconState, d : Deposit)  returns (s' : BeaconState)  
-    //     requires |s.validators| + 1 <= VALIDATOR_REGISTRY_LIMIT as int
-    //     requires s.eth1_deposit_index as int + 1 < 0x10000000000000000 
-    //     requires |s.validators| == |s.balances|
-    //     requires total_balances(s.balances) + d.data.amount as int < 0x10000000000000000
-
-    //     ensures s'.eth1_deposit_index == s.eth1_deposit_index + 1
-    //     //ensures d.data.pubkey !in seqKeysInValidators(s.validators) ==> s'.validators == s.validators + [get_validator_from_deposit(d)]
-    //     //ensures d.data.pubkey in seqKeysInValidators(s.validators) ==> s'.validators == s.validators 
-    //     ensures s' == updateDeposit(s,d)
-
-    //     //ensures |s'.validators| == |s'.balances|        // maybe include in property lemmas
-    //     //ensures |s.validators| <= |s'.validators| <= |s.validators| + 1 // maybe include in property lemmas
-    //     //ensures |s.balances| <= |s'.balances| <= |s.balances| + 1 // maybe include in property lemmas
-    //     //ensures |s'.validators| <= VALIDATOR_REGISTRY_LIMIT
-        
-    // {
-    //     // note that it is assumed that all new validator deposits are verified
-    //     // ie the step # Verify the deposit signature (proof of possession) which is not checked by the deposit contract
-    //     // is not performed
-    //     var pk := seqKeysInValidators(s.validators);
-    //     s' := s.(
-    //             eth1_deposit_index := (s.eth1_deposit_index as int + 1) as uint64,
-    //             validators := if d.data.pubkey in pk then 
-    //                                 s.validators // unchanged validator members
-    //                             else 
-    //                                 (s.validators + [get_validator_from_deposit(d)]),
-    //             balances := if d.data.pubkey in pk then 
-    //                                 individualBalanceBoundMaintained(s.balances,d);
-    //                                 increase_balance(s,get_validator_index(pk, d.data.pubkey),d.data.amount).balances
-    //                             else 
-    //                                 s.balances + [d.data.amount]
-    //     );
-    // }
-
-    // /**
-    //  *  
-    //  *  @note       This method uses PendingAttestations instead of attestations in the 
-    //  *              input parameter `xa`.The difference is in the signature field which 
-    //  *              we omit in this foirst-cut.
-    //  */
-    //  method process_attestations(s: BeaconState, xa: ListOfAttestations)  returns (s' : BeaconState)
-    //     // requires 
-    //     ensures s' == s  
-    //  {
-    //      return s;
-    //  }
-     
-
-    // predicate isValidAttestationInState(s: BeaconState, a: PendingAttestation)
-    // {
-    //     && get_previous_epoch(s) <= a.data.target.epoch <= get_current_epoch(s)
-    //     && a.data.target.epoch == compute_epoch_at_slot(a.data.slot)
-    //     //  attestation is not too recent
-    //     && a.data.slot as nat + MIN_ATTESTATION_INCLUSION_DELAY as nat <= s.slot as nat  
-    //     //  attestation is not old
-    //     && a.data.slot as nat + SLOTS_PER_EPOCH as nat >= s.slot as nat 
-    //     //  if attestation target is current epoch, then the source must
-    //     //  be the current justified checkpoint
-    //     && (a.data.target.epoch == get_current_epoch(s) ==> 
-    //         a.data.source == s.current_justified_checkpoint)
-    //     //  if attestation target is previous epoch, then the source must
-    //     //  be the the previous justified checkpoint
-    //     && (a.data.target.epoch == get_previous_epoch(s) ==> 
-    //         a.data.source == s.previous_justified_checkpoint)
-        
-    // }
-    
+    }   
     
 }
