src/dafny/beacon/statetransition/StateTransition.s.dfy
@@ -12,18 +12,19 @@
  * under the License.
  */
 
-include "../../utils/NativeTypes.dfy"
 include "../../utils/Eth2Types.dfy"
 include "../../utils/Helpers.dfy"
-include "../../utils/MathHelpers.dfy"
 include "../../ssz/Constants.dfy"
 include "../BeaconChainTypes.dfy"
 include "../validators/Validators.dfy"
 include "../attestations/AttestationsTypes.dfy"
 include "../attestations/AttestationsHelpers.dfy"
 include "../Helpers.dfy"
+include "../Helpers.s.dfy"
 include "EpochProcessing.s.dfy"
 include "ProcessOperations.s.dfy"
+include "ProcessOperations.dfy"
+include "StateTransition.p.dfy"
 
 /**
  * State transition functional specification for the Beacon Chain.
@@ -31,7 +32,6 @@ include "ProcessOperations.s.dfy"
 module StateTransitionSpec {
     
     //  Import some constants, types and beacon chain helpers.
-    import opened NativeTypes
     import opened Eth2Types
     import opened Constants
     import opened BeaconChainTypes
@@ -39,123 +39,14 @@ module StateTransitionSpec {
     import opened AttestationsTypes
     import opened AttestationsHelpers
     import opened BeaconHelpers
-    import opened MathHelpers
+    import opened BeaconHelperSpec
     import opened EpochProcessingSpec
     import opened ProcessOperationsSpec
-    
+    import opened ProcessOperations
+    import opened StateTransitionProofs
 
-    
     
     //  Specifications of finalisation of a state and forward to future slot.
-
-    /**
-     *  Result of processing eth1Data.
-     *  
-     *  @param  s   A state.
-     *  @param  b   A block body to process.
-     *  @returns    The state `s` updated to include b.eth1_data in the list of votes
-     *              and state `s` eth1_data field set to b.eth1_data if b.eth1_data has
-     *              received more than 1/2 * (EPOCHS_PER_ETH1_VOTING_PERIOD * SLOTS_PER_EPOCH) votes.
-     */
-    function updateEth1Data(s: BeaconState, b: BeaconBlockBody) :  BeaconState 
-        requires |s.validators| == |s.balances| 
-        requires |s.eth1_data_votes| < EPOCHS_PER_ETH1_VOTING_PERIOD as int * SLOTS_PER_EPOCH as int
-        ensures |updateEth1Data(s,b).validators| == |updateEth1Data(s,b).balances|
-        ensures updateEth1Data(s,b).eth1_deposit_index == s.eth1_deposit_index
-        ensures updateEth1Data(s,b).validators == s.validators
-        ensures updateEth1Data(s,b).balances == s.balances
-    {
-        s.( eth1_data_votes := s.eth1_data_votes + [b.eth1_data],
-            eth1_data := if (count_eth1_data_votes(s.eth1_data_votes + [b.eth1_data], b.eth1_data) * 2) > (EPOCHS_PER_ETH1_VOTING_PERIOD * SLOTS_PER_EPOCH) as int 
-                then b.eth1_data 
-                else s.eth1_data
-            )
-    }
-
-    /**
-     *  Result of processing a block.
-     *  
-     *  @param  s   A state.
-     *  @param  b   A block to add to the state `s`.
-     *  @returns    The state `s` updated to point to `b` with state_root set to 0.
-     */
-    function addBlockToState(s: BeaconState, b: BeaconBlock) :  BeaconState 
-        //  Verify that the slots match
-        requires b.slot == s.slot  
-        // Verify that the parent matches
-        requires b.parent_root == hash_tree_root(s.latest_block_header) 
-        requires |s.validators| == |s.balances| 
-        ensures |addBlockToState(s,b).validators| == |addBlockToState(s,b).balances|
-        ensures addBlockToState(s,b).eth1_data_votes == s.eth1_data_votes
-        // ensures |addBlockToState(s,b).eth1_data_votes| == |s.eth1_data_votes|
-        ensures addBlockToState(s,b).eth1_deposit_index == s.eth1_deposit_index
-        ensures addBlockToState(s,b).validators == s.validators
-        ensures addBlockToState(s,b).balances == s.balances
-    {
-        s.(
-            latest_block_header := BeaconBlockHeader(
-                b.slot,
-                b.proposer_index,
-                b.parent_root,
-                DEFAULT_BYTES32
-            )
-        )
-    }
-
-    /**
-     *  Complete the current slot.
-     *
-     *  @param  s   A beacon state.
-     *  @returns    A new state `s' such that:
-     *              1. a new latest_block_header' state_root set to the hash_tree_root(s) 
-     *              2. the hash_tree_root(s) archived in the s'.state_roots for the slot
-     *              3. the hash_tree_root of the new_block_header is archived 
-     *              in s'.block_roots
-     */
-    function resolveStateRoot(s: BeaconState): BeaconState 
-        //  Make sure s.slot does not  overflow
-        requires s.slot as nat + 1 < 0x10000000000000000 as nat
-        requires minimumActiveValidators(s)
-
-        //  parent_root of the state block header is preserved
-        ensures s.latest_block_header.parent_root == resolveStateRoot(s).latest_block_header.parent_root
-        //  eth1_deposit_index is left unchanged
-        ensures s.eth1_deposit_index == resolveStateRoot(s).eth1_deposit_index
-        //  eth1_data_votes unchanged
-        ensures s.eth1_data_votes == resolveStateRoot(s).eth1_data_votes
-        //  previous_epoch_attestations unchanged
-        ensures s.previous_epoch_attestations == resolveStateRoot(s).previous_epoch_attestations
-
-        ensures  s.latest_block_header.state_root != DEFAULT_BYTES32 ==>
-            resolveStateRoot(s) == advanceSlot(s)
-        
-        ensures minimumActiveValidators(resolveStateRoot(s))
-    {
-        var new_latest_block_header := 
-            if (s.latest_block_header.state_root == DEFAULT_BYTES32 ) then 
-                s.latest_block_header.(state_root := hash_tree_root(s))
-            else 
-                s.latest_block_header
-            ;
-        //  new state
-        var s' := s.(
-                slot := s.slot + 1,
-                latest_block_header := new_latest_block_header,
-                block_roots := s.block_roots[(s.slot % SLOTS_PER_HISTORICAL_ROOT) as int := hash_tree_root(new_latest_block_header)],
-                state_roots := s.state_roots[(s.slot % SLOTS_PER_HISTORICAL_ROOT) as int := hash_tree_root(s)]
-            );
-        SetMinimumNumberOfValidators(s');
-        s'
-    }
-
-    // Property of s.previous_epoch_attestations that must be maintained
-    // Need to create a proof that shows PendingAttestations must always follow these rules
-    lemma PreviousEpochAttestationsProperties(s: BeaconState)
-        requires |s.validators| == |s.balances|
-        ensures forall a :: a in s.previous_epoch_attestations ==> a.data.index < get_committee_count_per_slot(s, compute_epoch_at_slot(a.data.slot)) <= TWO_UP_6 
-        ensures forall a :: a in s.previous_epoch_attestations ==> TWO_UP_5 as nat <= |get_active_validator_indices(s.validators, compute_epoch_at_slot(a.data.slot))| <= TWO_UP_11 as nat * TWO_UP_11 as nat 
-        ensures forall a :: a in s.previous_epoch_attestations ==> 0 < |get_beacon_committee(s, a.data.slot, a.data.index)| == |a.aggregation_bits| <= MAX_VALIDATORS_PER_COMMITTEE as nat 
-    //{} 
 
     /**
      *  Finalise a state and forward to slot in the future.
@@ -190,33 +81,7 @@ module StateTransitionSpec {
             PreviousEpochAttestationsProperties(s1);
             nextSlot(s1)
     }
-
-    /**
-     *  Advance a state by one slot.
-     *
-     *  @param  s   A beacon state.
-     *  @returns    The successor state for `slot + 1`.
-     *
-     *  @note       This function increment the slot number and archives 
-     *              the previous state_root and block_root, and copy verbatim the 
-     *              latest_block_header.
-     */
-    function advanceSlot(s : BeaconState) : BeaconState 
-        //  Make sure s.slot does not overflow
-        requires s.slot as nat + 1 < 0x10000000000000000 as nat
-    {
-        //  Add header root to history of block_roots
-        var new_block_roots := s.block_roots[(s.slot % SLOTS_PER_HISTORICAL_ROOT) as int := hash_tree_root(s.latest_block_header)];
-        //  Add state root to history of state roots
-        var new_state_roots := s.state_roots[(s.slot % SLOTS_PER_HISTORICAL_ROOT) as int := hash_tree_root(s)];
-        //  Increment slot and copy latest_block_header
-        s.(
-            slot := s.slot + 1,
-            block_roots := new_block_roots,
-            state_roots := new_state_roots
-        )
-    }
-
+    
     /**
      *  Defines the value of state at next slot.
      */
@@ -273,12 +138,246 @@ module StateTransitionSpec {
                 resolveStateRoot(s)
     }
 
-    lemma SetMinimumNumberOfValidators(s: BeaconState)
-        ensures minimumActiveValidators(s)
-    // It is assumed that there will always be at least one active validator
-    // An alternative to this assumption lemma would be to add preconditions to assert that the number of
-    // active validators cannot drop to zero.
+    
+    /**
+     *  Complete the current slot.
+     *
+     *  @param  s   A beacon state.
+     *  @returns    A new state `s' such that:
+     *              1. a new latest_block_header' state_root set to the hash_tree_root(s) 
+     *              2. the hash_tree_root(s) archived in the s'.state_roots for the slot
+     *              3. the hash_tree_root of the new_block_header is archived 
+     *              in s'.block_roots
+     */
+    function resolveStateRoot(s: BeaconState): BeaconState 
+        //  Make sure s.slot does not  overflow
+        requires s.slot as nat + 1 < 0x10000000000000000 as nat
+        requires minimumActiveValidators(s)
 
+        //  parent_root of the state block header is preserved
+        ensures s.latest_block_header.parent_root == resolveStateRoot(s).latest_block_header.parent_root
+        //  eth1_deposit_index is left unchanged
+        ensures s.eth1_deposit_index == resolveStateRoot(s).eth1_deposit_index
+        //  eth1_data_votes unchanged
+        ensures s.eth1_data_votes == resolveStateRoot(s).eth1_data_votes
+        //  previous_epoch_attestations unchanged
+        ensures s.previous_epoch_attestations == resolveStateRoot(s).previous_epoch_attestations
+
+        ensures  s.latest_block_header.state_root != DEFAULT_BYTES32 ==>
+            resolveStateRoot(s) == advanceSlot(s)
+        
+        ensures minimumActiveValidators(resolveStateRoot(s))
+    {
+        var new_latest_block_header := 
+            if (s.latest_block_header.state_root == DEFAULT_BYTES32 ) then 
+                s.latest_block_header.(state_root := hash_tree_root(s))
+            else 
+                s.latest_block_header
+            ;
+        //  new state
+        var s' := s.(
+                slot := s.slot + 1,
+                latest_block_header := new_latest_block_header,
+                block_roots := s.block_roots[(s.slot % SLOTS_PER_HISTORICAL_ROOT) as int := hash_tree_root(new_latest_block_header)],
+                state_roots := s.state_roots[(s.slot % SLOTS_PER_HISTORICAL_ROOT) as int := hash_tree_root(s)]
+            );
+        SetMinimumNumberOfValidators(s');
+        s'
+    }
+
+    
+
+    
+
+    /**
+     *  Advance a state by one slot.
+     *
+     *  @param  s   A beacon state.
+     *  @returns    The successor state for `slot + 1`.
+     *
+     *  @note       This function increment the slot number and archives 
+     *              the previous state_root and block_root, and copy verbatim the 
+     *              latest_block_header.
+     */
+    function advanceSlot(s : BeaconState) : BeaconState 
+        //  Make sure s.slot does not overflow
+        requires s.slot as nat + 1 < 0x10000000000000000 as nat
+    {
+        //  Add header root to history of block_roots
+        var new_block_roots := s.block_roots[(s.slot % SLOTS_PER_HISTORICAL_ROOT) as int := hash_tree_root(s.latest_block_header)];
+        //  Add state root to history of state roots
+        var new_state_roots := s.state_roots[(s.slot % SLOTS_PER_HISTORICAL_ROOT) as int := hash_tree_root(s)];
+        //  Increment slot and copy latest_block_header
+        s.(
+            slot := s.slot + 1,
+            block_roots := new_block_roots,
+            state_roots := new_state_roots
+        )
+    }
+
+
+    //  Specifications of block processing.
+    
+    /**
+     *  Whether a block is valid in a given state.
+     *
+     *  @param  s   A beacon state.
+     *  @param  b   A block.
+     *
+     *  @returns    true iff `b` can be successfully added to the state `s`.
+     */
+    predicate isValidBlock(s : BeaconState, b : BeaconBlock) 
+    {
+        //  The block slot should be in the future.
+        s.slot < b.slot 
+        //  Fast forward s to b.slot and check `b` can be attached to the
+        //  resulting state's latest_block_header.
+        //  Check that number of deposits in b.body can be processed
+        && s.eth1_deposit_index as int + |b.body.deposits| < 0x10000000000000000  
+        && |s.validators| + |b.body.deposits| <= VALIDATOR_REGISTRY_LIMIT as int
+        // note that |b.body.deposits| is larger than required, only existing + new validators need to obey this bound
+        && total_balances(s.balances) + total_deposits(b.body.deposits) < 0x10000000000000000
+        // note that the |b.body.deposits| and total_deposits should refer to valid deposits
+        && |s.validators| == |s.balances|
+        && |s.eth1_data_votes| < EPOCHS_PER_ETH1_VOTING_PERIOD as int * SLOTS_PER_EPOCH as int
+        // && b.parent_root == 
+        //     hash_tree_root(
+        //         forwardStateToSlot(nextSlot(s), 
+        //         b.slot
+        //     ).latest_block_header) 
+        // //  Check that the block provides the correct hash for the state.
+        // &&  b.state_root == hash_tree_root(
+        //         updateDeposits(
+        //             updateEth1Data(
+        //                 addBlockToState(
+        //                     forwardStateToSlot(nextSlot(s), b.slot), 
+        //                     b
+        //                 ),
+        //                 b.body),
+        //             b.body.deposits
+        //         )
+        //     )
+    }
+
+    /** */
+    function updateBlock(s: BeaconState, b: BeaconBlock): BeaconState
+        requires b.slot == s.slot
+        requires b.parent_root == hash_tree_root(s.latest_block_header)
+        requires s.eth1_deposit_index as int + |b.body.deposits| < 0x10000000000000000  
+        requires |s.eth1_data_votes| < EPOCHS_PER_ETH1_VOTING_PERIOD as int * SLOTS_PER_EPOCH as int
+        requires |s.validators| == |s.balances|
+        requires |s.validators| + |b.body.deposits| <= VALIDATOR_REGISTRY_LIMIT as int
+        requires total_balances(s.balances) + total_deposits(b.body.deposits) < 0x10000000000000000
+        requires |get_active_validator_indices(s.validators, get_current_epoch(s))| > 0
+        requires isValidBeaconBlockBody(s, b.body)
+
+        // ensures updateBlock(s,b).slot == b.slot
+        // ensures updateBlock(s,b).latest_block_header == BeaconBlockHeader(b.slot, b.proposer_index, b.parent_root, DEFAULT_BYTES32)
+        // ensures |updateBlock(s,b).validators| == |updateBlock(s,b).balances|
+        //ensures updateBlock(s,b) == updateOperations(updateEth1Data(updateRandao(addBlockToState(s, b), b.body), b.body), b.body)
+        
+    {
+        //  Start by creating a block header from the ther actual block.
+        var s1 := addBlockToState(s, b); 
+        assert s1 == addBlockToState(s, b);
+        assert (s1.balances == s.balances);
+        assert (s1.validators == s.validators);
+        
+        var s2 := updateRandao(s1, b.body);
+        assert s2 == updateRandao(addBlockToState(s, b), b.body);
+        assert (s2.balances == s.balances);
+        assert (s2.validators == s.validators);
+        
+        var s3 := updateEth1Data(s2, b.body);
+        assert (s3.balances == s.balances);
+        assert (s3.validators == s.validators);
+        assert |s3.validators| == |s3.balances|;
+        assert s3 == updateEth1Data(updateRandao(addBlockToState(s, b), b.body), b.body);
+
+        assert |get_active_validator_indices(s3.validators, get_current_epoch(s3))| > 0;
+        assume isValidBeaconBlockBody(s3, b.body);
+        
+        var s4 := updateOperations(s3, b.body);
+        assert s4 == updateOperations(updateEth1Data(updateRandao(addBlockToState(s, b), b.body), b.body), b.body);
+        s4
+    }
+
+    
+    /**
+     *  Result of processing a block.
+     *  
+     *  @param  s   A state.
+     *  @param  b   A block to add to the state `s`.
+     *  @returns    The state `s` updated to point to `b` with state_root set to 0.
+     */
+    function addBlockToState(s: BeaconState, b: BeaconBlock) :  BeaconState 
+        //  Verify that the slots match
+        requires b.slot == s.slot  
+        // Verify that the parent matches
+        requires b.parent_root == hash_tree_root(s.latest_block_header) 
+        requires |s.validators| == |s.balances| 
+        ensures |addBlockToState(s,b).validators| == |addBlockToState(s,b).balances|
+        ensures addBlockToState(s,b).eth1_data_votes == s.eth1_data_votes
+        // ensures |addBlockToState(s,b).eth1_data_votes| == |s.eth1_data_votes|
+        ensures addBlockToState(s,b).eth1_deposit_index == s.eth1_deposit_index
+        ensures addBlockToState(s,b).validators == s.validators
+        ensures addBlockToState(s,b).balances == s.balances
+    {
+        s.(
+            latest_block_header := BeaconBlockHeader(
+                b.slot,
+                b.proposer_index,
+                b.parent_root,
+                DEFAULT_BYTES32
+            )
+        )
+    }
+
+
+    /** */
+    function updateRandao(s: BeaconState, b: BeaconBlockBody) : BeaconState
+        requires |s.validators| == |s.balances|
+        ensures |updateRandao(s,b).validators| == |updateRandao(s,b).balances|
+        ensures updateRandao(s,b) == s.(randao_mixes := updateRandao(s,b).randao_mixes)
+        ensures updateRandao(s,b).latest_block_header == s.latest_block_header
+    {
+        var epoch := get_current_epoch(s);
+
+        // Verify RANDAO reveal not implemented
+        //var proposer := s.validators[get_beacon_proposer_index(s)];
+        // signing_root = compute_signing_root(epoch, get_domain(state, DOMAIN_RANDAO))
+        // assert bls.Verify(proposer.pubkey, signing_root, body.randao_reveal)
+
+        // # Mix in RANDAO reveal (use simplified mix value)
+        var mix := DEFAULT_BYTES32; //var mix := xor(get_randao_mix(s, epoch), hash(b.randao_reveal));
+        s.(randao_mixes := s.randao_mixes[(epoch % EPOCHS_PER_HISTORICAL_VECTOR) as nat := mix])
+    }
+
+
+    /**
+     *  Result of processing eth1Data.
+     *  
+     *  @param  s   A state.
+     *  @param  b   A block body to process.
+     *  @returns    The state `s` updated to include b.eth1_data in the list of votes
+     *              and state `s` eth1_data field set to b.eth1_data if b.eth1_data has
+     *              received more than 1/2 * (EPOCHS_PER_ETH1_VOTING_PERIOD * SLOTS_PER_EPOCH) votes.
+     */
+    function updateEth1Data(s: BeaconState, b: BeaconBlockBody) :  BeaconState 
+        requires |s.validators| == |s.balances| 
+        requires |s.eth1_data_votes| < EPOCHS_PER_ETH1_VOTING_PERIOD as int * SLOTS_PER_EPOCH as int
+        ensures |updateEth1Data(s,b).validators| == |updateEth1Data(s,b).balances|
+        ensures updateEth1Data(s,b).eth1_deposit_index == s.eth1_deposit_index
+        ensures updateEth1Data(s,b).validators == s.validators
+        ensures updateEth1Data(s,b).balances == s.balances
+    {
+        s.( eth1_data_votes := s.eth1_data_votes + [b.eth1_data],
+            eth1_data := if (count_eth1_data_votes(s.eth1_data_votes + [b.eth1_data], b.eth1_data) * 2) > (EPOCHS_PER_ETH1_VOTING_PERIOD * SLOTS_PER_EPOCH) as int 
+                then b.eth1_data 
+                else s.eth1_data
+            )
+    }
+    
     
 
     /**
